mm0-lean/hoare.lean
@@ -1,0 +1,517 @@
+import x86 data.set.lattice data.list.basic tactic.sanity_check
+
+
+namespace x86
+
+inductive flag_place | CFP | ZFP | SFP | OFP
+
+def flag_place.read (f : flags) : flag_place → bool
+| flag_place.CFP := f.CF
+| flag_place.ZFP := f.ZF
+| flag_place.SFP := f.SF
+| flag_place.OFP := f.OF
+
+def flag_place.write (f : flags) (b : bool) : flag_place → flags
+| flag_place.CFP := {CF := b, ..f}
+| flag_place.ZFP := {ZF := b, ..f}
+| flag_place.SFP := {SF := b, ..f}
+| flag_place.OFP := {OF := b, ..f}
+
+inductive place
+| flag : flag_place → place
+| reg : regnum → place
+| rip : place
+| mem : qword → place
+
+inductive place.read (k : config) : place → ∀ {n}, bitvec n → Prop
+| flag {f} : place.read (place.flag f) (bitvec.singleton (f.read k.flags))
+| reg {r} : place.read (place.reg r) (k.regs r)
+| rip : place.read place.rip k.rip
+| mem {a b} : k.mem.read1 perm.R a b → place.read (place.mem a) b
+
+inductive place.write (k : config) : place → ∀ {n}, bitvec n → config → Prop
+| flag {f b} : place.write (place.flag f) (bitvec.singleton b) {flags := f.write k.flags b, ..k}
+| reg {r n q} : place.write (place.reg r) q (k.write_reg r n q)
+| rip {q} : place.write place.rip q {rip := q, ..k}
+| mem {a b m'} : k.mem.write1 a b m' → place.write (place.mem a) b {mem := m', ..k}
+
+def split (H h₁ h₂ : set place) : Prop :=
+H = h₁ ∪ h₂ ∧ disjoint h₁ h₂
+
+def sProp := config → set place → Prop
+
+def sProp.sep (P Q : sProp) : sProp :=
+λ k H, ∃ H₁ H₂, split H H₁ H₂ ∧ P k H₁ ∧ Q k H₂
+
+instance : has_mul sProp := ⟨sProp.sep⟩
+
+def sProp.wand (P Q : sProp) : sProp :=
+λ k H₂, ∀ H₁ H, split H H₁ H₂ → P k H₁ → Q k H
+
+def sProp.mk (H : config → set place) : sProp := λ k, eq (H k)
+
+def sProp.reserve (S : set place) : sProp :=
+sProp.mk $ λ k, {p | p ∈ S ∧ ∃ n v, @place.read k p n v}
+
+def emp : sProp := sProp.mk $ λ _, ∅
+
+def lift' (p : config → Prop) : sProp := λ k _, p k
+
+def lift (p : Prop) : sProp := λ _ _, p
+
+def sProp.and (P Q : sProp) : sProp := λ k H, P k H ∧ Q k H
+
+def sProp.or (P Q : sProp) : sProp := λ k H, P k H ∨ Q k H
+
+def sProp.with' (p : sProp) (q : config → Prop) : sProp := p.and (lift' q)
+def sProp.with (p : sProp) (q : Prop) : sProp := p.and (lift q)
+def liftE (p : Prop) : sProp := sProp.with emp p
+
+def sProp.sn (p : place) {n} (v : bitvec n) : sProp :=
+sProp.mk $ λ k, {p' | p = p' ∧ p.read k v}
+
+def sProp.ex {α} (p : α → sProp) : sProp := λ k H, ∃ a, p a k H
+
+def sProp.al {α} (p : α → sProp) : sProp := λ k H, ∀ a, p a k H
+
+def sProp.flags (f : flags) : sProp :=
+sProp.al $ λ p : flag_place,
+sProp.sn (place.flag p) (bitvec.singleton $ p.read f)
+
+inductive block
+| reg : regnum → wsize → block
+| mem : qword → qword → block
+| const : list byte → block
+
+def block.size : block → qword
+| (block.reg _ sz) := (sz.to_nat / 8 : ℕ)
+| (block.mem _ sz) := sz
+| (block.const l) := l.length
+
+inductive block.places : block → set place
+| reg {r sz} : block.places (block.reg r sz) (place.reg r)
+| mem {a b sz : qword} :
+  (bitvec.sub b a).to_nat ≤ sz.to_nat →
+  block.places (block.mem a sz) (place.mem b)
+
+def block.disj (b1 b2 : block) := disjoint b1.places b2.places
+
+def sProp.mem_block (p : perm) (a : qword) (v : list byte) : sProp :=
+(sProp.reserve (block.mem a v.length).places).with' $ λ k, k.mem.read' p a v
+
+def sProp.block : block → list byte → sProp
+| (block.reg r sz) v :=
+  (sProp.reserve (block.reg r sz).places).with' $ λ k,
+    read_full_imm sz (k.regs r) v
+| (block.mem a sz) v :=
+  (sProp.reserve (block.mem a sz).places).with' $ λ k,
+    k.mem.read a v ∧ v.length = sz.to_nat
+| (block.const l) v := liftE $ v = l
+
+def sProp.block_writable : block → sProp
+| (block.reg r sz) := sProp.reserve (block.reg r sz).places
+| (block.mem a sz) :=
+  (sProp.reserve (block.mem a sz).places).with' $ λ k,
+    ∃ v, k.mem.read' perm.W a v ∧ v.length = sz.to_nat
+| (block.const _) := lift false
+
+def locals_ctx (n : ℕ) := {Γ : list (ℕ × block) //
+  Γ.pairwise (λ i j, i.1 ≠ j.1 ∧ i.2.disj j.2) ∧
+  ∀ i : ℕ × block, i ∈ Γ → i.1 < n}
+
+instance {n} : has_mem (ℕ × block) (locals_ctx n) := ⟨λ a Γ, a ∈ Γ.1⟩
+
+def locals_ctx.cons {n} (Γ : locals_ctx n) (b : block)
+  (h : ∀ i : ℕ × block, i ∈ Γ → b.disj i.2) : locals_ctx (n+1) :=
+⟨(n, b) :: Γ.1,
+  list.pairwise_cons.2 ⟨λ i h', ⟨ne_of_gt $ Γ.2.2 _ h', h _ h'⟩, Γ.2.1⟩,
+  by rintro i (rfl|h'); [
+    apply nat.lt_succ_self,
+    exact nat.lt_succ_of_lt (Γ.2.2 _ h')]⟩
+
+def locals_ctx.shrink {m n} (Γ : locals_ctx m) : locals_ctx n :=
+⟨Γ.1.filter (λ i, i.1 < n),
+  list.pairwise_of_sublist (list.filter_sublist _) Γ.2.1,
+  λ i h, (list.mem_filter.1 h).2⟩
+
+def labels_ctx := qword × list qword
+
+def labels_ctx.cons (q : qword) (L : labels_ctx) : labels_ctx :=
+⟨L.1, q :: L.2⟩
+
+inductive hoare_p (Q : kcfg → set place → Prop) : kcfg → set place → Prop
+| zero {{k H}} : Q k H → hoare_p k H
+| step {{k H}} : (∃ k', kcfg.step k k') →
+  (∀ k', k.step k' → hoare_p k' H) → hoare_p k H
+| exit (k : kcfg) (H ret) :
+  k.k.exit ret → (ret = 0 → Q k H) → hoare_p k H
+
+def hoare (P Q : kcfg → set place → Prop) :=
+∀ {{k H}}, P k H → hoare_p Q k H
+
+def sHoareIO (P : sProp) (Q : list byte → list byte → sProp) :=
+∀ {{i o}}, hoare (λ k H, P k.k H ∧ k.input = i ∧ k.output = o)
+  (λ k H, ∃ i' o', i = i' ++ k.input ∧ o = k.output ++ o' ∧
+    (Q i' o') k.k H)
+
+def noIO (Q : sProp) (i o : list byte) : sProp := Q.with (i = [] ∧ o = [])
+def sHoare (P Q : sProp) := sHoareIO P (noIO Q)
+
+inductive exit_kind
+| straight
+| label (n : ℕ)
+
+def exit_kind.result (L : labels_ctx) (pos : qword) : exit_kind → sProp
+| exit_kind.straight := sProp.sn place.rip pos
+| (exit_kind.label n) := sProp.ex $ λ h, sProp.sn place.rip (L.2.nth_le n h)
+
+def stmt (n) :=
+labels_ctx → locals_ctx n →
+∀ rip : qword, list byte → Prop
+
+def stmt.hoareIO (P : sProp) {n} (C : stmt n)
+  (Q : exit_kind → list byte → list byte → sProp) : Prop :=
+∀ L Γ rip l, C L Γ rip l →
+  sHoareIO (P * sProp.sn place.rip rip *
+      sProp.mem_block (perm.R + perm.X) rip l)
+    (λ i o,
+      ((sProp.sn place.rip L.1).or $
+        sProp.ex $ λ e, Q e i o * e.result L (rip + l.length)) *
+      sProp.mem_block (perm.R + perm.X) rip l)
+
+def stmt.hoare (P : sProp) {n} (C : stmt n) (Q : exit_kind → sProp) : Prop :=
+stmt.hoareIO P C (λ e, noIO (Q e))
+
+def hstmt {n} (P : sProp) (Q : sProp) : stmt n :=
+λ L Γ rip v,
+  sHoare (P * sProp.sn place.rip rip * sProp.mem_block (perm.R + perm.X) rip v)
+    (Q * sProp.sn place.rip (rip + v.length) * sProp.mem_block (perm.R + perm.X) rip v)
+
+def stmt.all {α n} (s : α → stmt n) : stmt n :=
+λ L Γ rip v, ∀ a, s a L Γ rip v
+
+def stmt.ex {α n} (s : α → stmt n) : stmt n :=
+λ L Γ rip v, ∃ a, s a L Γ rip v
+
+def stmt.with {n} (p : Prop) (s : stmt n) : stmt n :=
+stmt.ex $ λ h : p, s
+
+def stmt.or {n} (s₁ s₂ : stmt n) : stmt n :=
+λ L Γ rip v, s₁ L Γ rip v ∨ s₂ L Γ rip v
+
+def stmt.lift {m n} (s : stmt n) : stmt m := λ L Γ, s L Γ.shrink
+
+def expr (n) := block → stmt n
+
+def expr.hoareIO (P : sProp) {n} (E : expr n)
+  (Q : list byte → list byte → list byte → sProp) : Prop :=
+∀ b, (E b).hoareIO (P * sProp.reserve b.places) $
+  λ e i o, exit_kind.cases_on e
+    (sProp.ex $ λ l, Q l i o * sProp.block b l)
+    (λ n, lift false)
+
+def expr.hoare (P : sProp) {n} (E : expr n) (Q : list byte → sProp) : Prop :=
+expr.hoareIO P E (λ ret, noIO (Q ret))
+
+def expr.lift {m n} (e : expr n) : expr m := λ b, stmt.lift (e b)
+
+class value (α : Type*) :=
+(size : ℕ)
+(eval : α → list byte → Prop)
+(eq_size : ∀ {v a}, eval a v → v.length = size)
+
+class type (α : Type*) :=
+(size : ℕ)
+(eval : α → list byte → sProp)
+(eq_size : ∀ {a v k H}, eval a v k H → v.length = size)
+
+def type.evalB {α} [type α] (a : α) (b : block) : sProp :=
+sProp.ex $ λ v, sProp.block b v * type.eval a v
+
+instance (α) [value α] : type α :=
+⟨value.size α, λ a v, lift $ value.eval a v, λ a v k H, value.eq_size⟩
+
+def expr.hoareT (P : sProp) {n} (E : expr n) {α} [type α] (Q : α → sProp) : Prop :=
+expr.hoare P E (λ v, sProp.ex $ λ a, Q a * type.eval a v)
+
+theorem bits_to_byte_length {n m w v} : @bits_to_byte n m w v → v.length = m :=
+by rintro ⟨bs⟩; exact bs.2
+
+def bits.value {n} (m : ℕ) : value (bitvec n) :=
+⟨m, bits_to_byte m, λ v a h, bits_to_byte_length h⟩
+
+instance unit.value : value unit :=
+⟨0, λ _ v, v = [], by rintro v _ ⟨⟩; refl⟩
+
+instance byte.value : value byte :=
+⟨1, λ b v, v = [b], by rintro v k ⟨⟩; refl⟩
+
+instance word.value : value word := bits.value 4
+instance qword.value : value qword := bits.value 8
+
+class box (α) [type α] := (deref : α)
+
+instance box.type (α) [type α] : type (box α) :=
+⟨8, λ x v, sProp.ex $ λ a, (sProp.ex $ λ l,
+    sProp.mem_block perm.R a l *
+    type.eval x.deref l).with (value.eval a v),
+  λ P v k H ⟨_, _, h⟩, bits_to_byte_length h⟩
+
+def const {n} (l : list byte) : expr n :=
+λ bl L Γ a v, bl = block.const l ∧ v = []
+
+def var {n} (i : ℕ) : expr n :=
+λ bl L Γ a v, (i, bl) ∈ Γ.1 ∧ v = []
+
+def hexpr {n} (P : sProp) (Q : block → sProp) : expr n :=
+λ ret, hstmt P (Q ret)
+
+def expr.all {α n} (e : α → expr n) : expr n :=
+λ ret, stmt.all $ λ a, e a ret
+
+def expr.ex {α n} (e : α → expr n) : expr n :=
+λ ret, stmt.ex $ λ a, e a ret
+
+def expr.with {n} (p : Prop) (s : expr n) : expr n :=
+expr.ex $ λ h : p, s
+
+def const' {n} (sz : wsize) (i : ℕ) : expr n :=
+expr.ex $ λ q, expr.ex $ λ l,
+expr.with (read_full_imm sz q l ∧ q.to_nat = i) $
+const l
+
+inductive stmt.seq {n} (s₁ : stmt n) (s₂ : stmt n) : stmt n
+| mk {L Γ rip v₁ v₂} :
+  s₁ L Γ rip v₁ →
+  s₂ L Γ (rip + v₁.length) v₂ →
+  stmt.seq L Γ rip (v₁ ++ v₂)
+
+inductive expr.bindS {n} (e₁ : expr n) (s₂ : block → stmt n) : stmt n
+| mk {b L Γ rip v₁ v₂} :
+  e₁ b L Γ rip v₁ →
+  s₂ b L Γ (rip + v₁.length) v₂ →
+  expr.bindS L Γ rip (v₁ ++ v₂)
+
+def expr.bind {n} (e₁ : expr n) (e₂ : block → expr n) : expr n :=
+λ b₂, expr.bindS e₁ $ λ b₁, e₂ b₁ b₂
+
+def expr.bindST {n α} [type α] (e₁ : expr n) (s₂ : α → stmt n) : stmt n :=
+expr.bindS e₁ $ λ b, stmt.all $ λ a : α,
+λ L Γ rip v, sHoare (type.evalB a b)
+  ((type.evalB a b).with (s₂ a L Γ rip v))
+
+def expr.bindT {n α} [type α] (e₁ : expr n) (e₂ : α → expr n) : expr n :=
+λ b₂, expr.bindST e₁ $ λ a, e₂ a b₂
+
+def block.mov {n} (dst src : block) : stmt n :=
+stmt.with (dst.size = src.size) $
+stmt.all $ λ val, hstmt
+  (sProp.block_writable dst * sProp.block src val)
+  (sProp.block dst val * sProp.block src val)
+
+def expr.set {n} (e₁ e₂ : expr n) : stmt n :=
+expr.bindS e₁ $ λ dst, expr.bindS e₂ $ block.mov dst
+
+inductive label | fail | label (n : ℕ)
+
+inductive label.loc (L : labels_ctx) : label → qword → Prop
+| fail : label.loc label.fail L.1
+| label (n h) : label.loc (label.label n) (L.2.nth_le n h)
+
+def stmt.jump_cc {n} (p : flags → bool) (l : label) : stmt n :=
+λ L Γ rip v, ∀ tgt, l.loc L tgt → ∀ f,
+sHoare (sProp.flags f * sProp.sn place.rip rip * sProp.mem_block (perm.R + perm.X) rip v)
+  (sProp.sn place.rip (cond (p f) tgt (rip + v.length)) * sProp.mem_block (perm.R + perm.X) rip v)
+
+def stmt.jump {n} : label → stmt n := stmt.jump_cc (λ _, tt)
+
+def boolexpr (n) := (flags → bool) × stmt n
+
+def boolexpr.hoare (P : sProp) {n} (E : boolexpr n) (Q : bool → sProp) : Prop :=
+stmt.hoare (P * sProp.reserve (set.range place.flag))
+  E.2
+  (λ e, exit_kind.cases_on e
+    (sProp.ex $ λ f, Q (E.1 f) * sProp.flags f)
+    (λ n, lift false))
+
+def boolexpr.not {n} (c : boolexpr n) : boolexpr n :=
+⟨λ f, bnot $ c.1 f, c.2⟩
+
+def boolexpr.jump_if {n} (c : boolexpr n) (l : label) : stmt n :=
+stmt.seq c.2 $ stmt.jump_cc c.1 l
+
+def stmt.nop {n} : stmt n := λ L Γ rip v, v = []
+
+def if_stmt {n} (c : boolexpr n) (s₁ s₂ : stmt n) : stmt n :=
+stmt.seq c.not.2 $ λ L Γ rip v,
+∃ v₁ v₂ v₃, v = v₁ ++ v₂ ++ v₃ ∧
+let q₁ := rip + v₁.length, q₂ := q₁ + v₂.length in
+stmt.jump_cc c.not.1 (label.label 0) (L.cons q₁) Γ rip v₁ ∧
+s₁.seq (stmt.jump (label.label 0)) (L.cons q₂) Γ q₁ v₂ ∧
+s₂.seq (stmt.jump (label.label 0)) (L.cons q₂) Γ q₂ v₃
+
+def loop {n} (s : stmt n) : stmt n :=
+λ L Γ rip, s (L.cons rip) Γ rip
+
+def block_stmt {n} (s : stmt n) : stmt n :=
+λ L Γ rip v, s (L.cons (rip + v.length)) Γ rip v
+
+def while {n} (c : boolexpr n) (s : stmt n) : stmt n :=
+block_stmt $ loop $
+  (c.not.jump_if (label.label 1)).seq $
+  s.seq $
+  stmt.jump (label.label 0)
+
+def decl_block {n} (b : block) (s : stmt (n + 1)) : stmt n :=
+λ L Γ rip v, ∀ h, s L (Γ.cons b h) rip v
+
+def decl {n} (sz : qword) (s : stmt (n + 1)) : stmt n :=
+λ L Γ rip v, ∀ b h, block.size b = sz → s L (Γ.cons b h) rip v
+
+def init_rvo {n} (sz : qword) (e : expr n) (s : stmt (n + 1)) : stmt n :=
+e.bindS $ λ b, stmt.with (b.size = sz) $
+λ L Γ rip v, ∃ h, s L (Γ.cons b h) rip v
+
+def init_assign {n} (sz : qword) (e : expr n) (s : stmt (n + 1)) : stmt n :=
+e.bindS $ λ b, stmt.with (b.size = sz) $
+decl sz $ ((var n).set e.lift).seq s
+
+def init {n} (sz : qword) (e : expr n) (s : stmt (n + 1)) : stmt n :=
+(init_rvo sz e s).or (init_assign sz e s)
+
+def for {n} (sz : qword) (start : expr n)
+  (test : boolexpr (n+1)) (incr body : stmt (n+1)) : stmt n :=
+init sz start $ while test $ body.seq incr
+
+def binop_expr {n α β γ} [type α] [type β]
+  (f : α → β → γ) (mk : γ → list byte → Prop)
+  (e₁ e₂ : expr n) : expr n :=
+e₁.bindT $ λ a : α, e₂.bindT $ λ b : β, 
+sorry
+
+def incr {n} (i) : stmt n :=
+(var i).set $ binop_expr (+) qword.to_list_byte (var i) (const [1])
+
+def bool_binop {n α β} [type α] [type β]
+  (f : α → β → bool) (e₁ e₂ : expr n) : boolexpr n :=
+⟨sorry, e₁.bindST $ λ a : α, e₂.bindST $ λ b : β,
+  sorry⟩
+
+def lt {n} (e₁ e₂ : expr n) : boolexpr n :=
+bool_binop (λ a b : qword, a.to_nat < b.to_nat) e₁ e₂
+
+def for_seq {n} (sz : qword) (max : expr n) (body : stmt (n+1)) : stmt n :=
+for sz (const' wsize.Sz64 0) (lt (const' wsize.Sz64 0) max.lift) (incr n) body
+
+----------------------------------------
+-- Assembly
+----------------------------------------
+
+theorem hoare.mono {P Q : kcfg → set place → Prop}
+  (H : ∀ {{k S}}, P k S → Q k S) : hoare P Q :=
+λ k S p, hoare_p.zero (H p)
+
+theorem hoare.step {P P' Q : kcfg → set place → Prop}
+  (h₁ : ∀ {{k S}}, P k S → ∃ k', k.step k')
+  (h₂ : ∀ {{k S}}, P k S → ∀ {{k'}}, k.step k' → P' k' S)
+  (h₃ : hoare P' Q) : hoare P Q :=
+λ k S p, hoare_p.step (h₁ p) (λ k' s, h₃ (h₂ p s))
+
+theorem hoare.mono_l {P P' Q : kcfg → set place → Prop}
+  (H : ∀ {{k S}}, P k S → P' k S) : hoare P' Q → hoare P Q :=
+λ H' k S h, H' (H h)
+
+theorem hoare_p.mono_l {P P' : kcfg → set place → Prop}
+  (H : ∀ {{k S}}, P k S → P' k S) {k S} : hoare_p P k S → hoare_p P' k S :=
+begin
+  intro h, induction h,
+  exact hoare_p.zero (H h_a),
+  exact hoare_p.step h_a (λ k', h_ih _),
+  exact hoare_p.exit _ _ _ h_a (λ e, H (h_a_1 e)),
+end
+
+theorem hoare.mono_r {P Q Q' : kcfg → set place → Prop}
+  (H : ∀ {{k S}}, Q k S → Q' k S) : hoare P Q → hoare P Q' :=
+λ H' k S h, hoare_p.mono_l H (H' h)
+
+theorem sHoareIO.mono {P : sProp} {Q : list byte → list byte → sProp}
+  (H : ∀ {{k S}}, P k S → Q [] [] k S) : sHoareIO P Q :=
+λ i o, hoare.mono $ by rintro k S ⟨h, rfl, rfl⟩; exact
+  ⟨[], [], rfl, (list.append_nil _).symm, H h⟩
+
+theorem sHoareIO.mono_l {P P' : sProp} {Q : list byte → list byte → sProp}
+  (H : ∀ {{k S}}, P k S → P' k S) : sHoareIO P' Q → sHoareIO P Q :=
+λ h i o, hoare.mono_l (by exact λ k S ⟨h₁, h₂⟩, ⟨H h₁, h₂⟩) (@h i o)
+
+theorem sHoareIO.mono_r {P : sProp} {Q Q' : list byte → list byte → sProp}
+  (H : ∀ {{i o k S}}, Q i o k S → Q' i o k S) : sHoareIO P Q → sHoareIO P Q' :=
+λ h i o, hoare.mono_r (by exact λ k S ⟨i', o', h₁, h₂, h₃⟩, 
+  ⟨i', o', h₁, h₂, H h₃⟩) (@h i o)
+
+theorem sHoareIO.step {P P' : sProp} {Q : list byte → list byte → sProp}
+  (h₁ : ∀ ⦃k i o S⦄, P k S → ∃ k', kcfg.step ⟨i, o, k⟩ k')
+  (h₂ : ∀ {{k₁ i₁ o₁ k₂ i₂ o₂ S}}, P k₁ S →
+    kcfg.step ⟨i₁, o₁, k₁⟩ ⟨i₂, o₂, k₂⟩ → P' k₂ S ∧ i₂ = i₁ ∧ o₂ = o₁)
+  (h₃ : sHoareIO P' Q) : sHoareIO P Q :=
+λ i o, hoare.step (λ ⟨i', o', k⟩ S h, h₁ h.1)
+  (by rintro ⟨i₁, o₁, k₁⟩ S ⟨h, rfl, rfl⟩ ⟨i₂, o₂, k₂⟩ h'; exact
+    @h₂ k₁ i₁ o₁ k₂ i₂ o₂ S h h')
+  (@h₃ i o)
+
+theorem sHoareIO.asm (P : sProp) (Q : list byte → list byte → sProp) :
+  sHoareIO P Q :=
+λ i o, _
+
+theorem sHoare.mono {P Q : sProp} (H : ∀ {{k S}}, P k S → Q k S) : sHoare P Q :=
+sHoareIO.mono $ λ k S h, ⟨H h, rfl, rfl⟩
+
+theorem sHoare.mono_l {P P' Q : sProp}
+  (H : ∀ {{k S}}, P k S → P' k S) : sHoare P' Q → sHoare P Q :=
+sHoareIO.mono_l H
+
+theorem sHoare.mono_r {P Q Q' : sProp}
+  (H : ∀ {{k S}}, Q k S → Q' k S) : sHoare P Q → sHoare P Q' :=
+sHoareIO.mono_r $ λ i o k S ⟨h₁, h₂⟩, ⟨H h₁, h₂⟩
+
+theorem config.isIO_terminal {k} :
+  (∃ k', config.step k k') → ¬ ∃ k', k.isIO k' := sorry
+
+theorem sHoare.step {P P' Q : sProp}
+  (h₁ : ∀ ⦃k S⦄, P k S → ∃ k', config.step k k')
+  (h₂ : ∀ ⦃k S⦄, P k S → ∀ k', config.step k k' → P' k' S) :
+  sHoare P' Q → sHoare P Q :=
+sHoareIO.step
+  (λ k i o S h, let ⟨k', h'⟩ := h₁ h in ⟨_, kcfg.step.noio h'⟩)
+  (λ k₁ i₁ o₁ k₂ i₂ o₂ S h h', begin
+    cases h', exact ⟨h₂ h _ h'_a, rfl, rfl⟩,
+    cases config.isIO_terminal (h₁ h) ⟨_, h'_a⟩
+  end)
+
+def stmt.asm {n} (s : stmt n) := Π L Γ rip, ∃ v, s L Γ rip v
+
+theorem hstmt.step {n} {P P' Q : sProp}
+  (h₁ : ∀ (L : labels_ctx) (Γ : locals_ctx n) rip,
+    ∃ l, ∀ v k S,
+    (P * sProp.sn place.rip rip *
+        sProp.mem_block (perm.R + perm.X) rip (l ++ v)) k S →
+    ∃ a k', decode a l ∧
+      (write_rip (k.rip + bitvec.of_nat 64 l.length) k).P () k' ∧
+      (execute a k').P () k ∧
+      ∀ H, P k H → P' k' H)
+  (h₂ : (@hstmt n P' Q).asm)
+  : (@hstmt n P Q).asm :=
+λ L Γ rip, let ⟨l, H⟩ := h₁ L Γ rip, ⟨v, H₂⟩ := h₂ L Γ rip in
+⟨l ++ v, begin
+  refine sHoare.step (λ k S h, _) (λ k S h k', _) (sHoare.mono_r _ H₂),
+  { rcases H v k S h with ⟨a, k', h₃, h₄, h₅, h₆⟩,
+    have : mem.readX (k.mem) (k.rip) l, sorry,
+    exact ⟨k, this, h₃, (), k', h₄, h₅⟩ },
+  { rintro ⟨l, a, _, m, d, h⟩,
+    sorry },
+  sorry,
+end⟩
+
+theorem hstmt.asm {n} (P : sProp) (Q : sProp) : (@hstmt n P Q).asm :=
+sorry
+
+end x86
